pcuic/theories/PCUICProgress.v
@@ -210,7 +210,7 @@ forall (P : global_env_ext -> context -> term -> term -> Type)
        forall pret : Σ ;;; Γ ,,, predctx |- p.(preturn) : tSort ps,
        P Σ (Γ ,,, predctx) p.(preturn) (tSort ps) ->
        PΓ Σ (Γ ,,, predctx) ->
-       is_allowed_elimination Σ ps idecl.(ind_kelim) ->
+       is_allowed_elimination Σ idecl.(ind_kelim) ps ->
        ctx_inst Σ Γ (p.(pparams) ++ indices)
          (List.rev (subst_instance p.(puinst) (mdecl.(ind_params) ,,, idecl.(ind_indices)))) ->
        PCUICTyping.ctx_inst P Σ Γ (p.(pparams) ++ indices) 
@@ -390,7 +390,7 @@ Lemma typing_ind_env `{cf : checker_flags} :
       forall pret : Σ ;;; Γ ,,, predctx |- p.(preturn) : tSort ps,
       P Σ (Γ ,,, predctx) p.(preturn) (tSort ps) ->
       PΓ Σ (Γ ,,, predctx) ->
-      is_allowed_elimination Σ ps idecl.(ind_kelim) ->
+      is_allowed_elimination Σ idecl.(ind_kelim) ps ->
       PCUICTyping.ctx_inst typing Σ Γ (p.(pparams) ++ indices)
         (List.rev (subst_instance p.(puinst) (mdecl.(ind_params) ,,, idecl.(ind_indices)))) ->
       PCUICTyping.ctx_inst P Σ Γ (p.(pparams) ++ indices) 
